Muda/Eqb.v
@@ -2,8 +2,6 @@
 From Stdlib Require Export Arith List Bool.
 Local Open Scope bool_scope.
 
-(** ** Boolean Equality Type Class *)
-
 Class Eqb (A : Type) := {
   eqb : A -> A -> bool
 }.
@@ -13,3 +11,10 @@ Class EqbSpec (A : Type) {eqb_instance : Eqb A} := {
 }.
 
 Notation "x =? y" := (eqb x y) (at level 70) : bool_scope.
+
+(* Optional: default boolean equality instance for nat *)
+#[export] Instance nat_eqb : Eqb nat := { eqb := Nat.eqb }.
+#[export] Instance nat_eqb_spec : EqbSpec nat.
+Proof.
+  constructor. apply Nat.eqb_eq.
+Qed.
