Muda/MUDA.v
@@ -1,5 +1,2 @@
-(** MUDA/MUDA.v 
-     Exports all MUDA protocol components.
-*)
-
+(** MUDA/MUDA.v **)
 From MUDA Require Export Eqb Types State Sorting Matching ClearingPrice Transitions.
